AG coind syntactic lemma

theories/CTree/Logic/AG.v
@@ -3,31 +3,57 @@ From Coq Require Import
   Classes.Morphisms.
 
 From Coinduction Require Import
-  coinduction lattice.
+  coinduction rel tactics.
 
 From CTree Require Import
   Events.Core
   CTree.Core
-  CTree.SBisim 
+  CTree.Equ
   CTree.Logic.Trans
   CTree.Logic.CanStep
   Logic.Ctl
   Logic.Kripke.
 
-Set Implicit Arguments.
 Generalizable All Variables.
 
-Import CTreeNotations CtlNotations.
+Import Ctree CTreeNotations CtlNotations.
 Local Open Scope ctl_scope.
 Local Open Scope ctree_scope.
 
 Section BasicLemmas.
-  Context {E: Type} {HE: Encode E} {X: Type} (φ: X -> World E -> Prop).
+  Context {E: Type} {HE: Encode E} {X: Type}.
 
-  Lemma ag_brS: forall n (k: fin' n -> ctree E X) w φ,
+  Lemma ag_vis: forall e (k: encode e -> ctree E X) (_ : encode e) w φ,
+      (vis_with φ w /\
+         forall (v: encode e), <( {k v}, {Obs e v} |= AG vis φ )>) <->
+        <( {Vis e k}, w |= AG vis φ )>.
+  Proof.
+    split; intros.
+    - destruct H as (Hd & H).
+      next; split.
+      + inv Hd.
+        now apply ctl_now.
+      + next; split; inv Hd.
+        * apply can_step_vis; auto with ctl.
+        * intros.
+          apply ktrans_vis in H0 as (i & -> & <- & ?).
+          apply H.
+    - next in H.
+      destruct H.      
+      next in H0.
+      destruct H0.
+      apply can_step_not_done in H0. 
+      split; auto.
+      intro v.
+      apply H1.
+      apply ktrans_vis.
+      exists v; auto.
+  Qed.
+  
+  Lemma ag_br: forall n (k: fin' n -> ctree E X) w φ,
       (not_done w /\
          forall (i: fin' n), <( {k i}, w |= AG now φ )>) <->
-        <( {BrS n k}, w |= AG now φ )>.
+        <( {Br n k}, w |= AG now φ )>.
   Proof.
     split; intros.
     - destruct H as (Hd & H).
@@ -37,9 +63,9 @@ Section BasicLemmas.
         destruct H.
         now cbn in *.
       + next; split.
-        * now apply can_step_brS.
+        * now apply can_step_br.
         * intros.
-          apply ktrans_brS in H0 as (i & ? & <- & ?).        
+          apply ktrans_br in H0 as (i & ? & <- & ?).        
           now rewrite H0.
     - next in H.
       destruct H.      
@@ -49,8 +75,32 @@ Section BasicLemmas.
       split; auto.
       intro i.
       apply H1.
-      apply ktrans_brS.
+      apply ktrans_br.
       exists i; auto.
+  Qed.
+
+  Lemma ag_ret: forall (x: X) w φ,      
+      <( {Ret x}, w |= AG φ )> -> False.
+  Proof.
+    intros. 
+    next in H.
+    destruct H.
+    next in H0; destruct H0.
+    destruct H0 as (t' & w' & TR).
+    cbn in TR, H1.
+    specialize (H1 _ _ TR).
+    dependent destruction TR; observe_equ x;
+      rewrite <- Eqt, H0 in H1; step in H1; inv H1; try contradiction;
+      destruct H3; apply can_step_not_done in H1; inv H1.
+  Qed.
+
+  Lemma ag_stuck: forall w φ,
+      <( {stuck: ctree E X}, w |= AG now φ )> -> False.
+  Proof.
+    intros.
+    next in H; destruct H.
+    next in H0; destruct H0.
+    now apply can_step_stuck in H0.
   Qed.
 End BasicLemmas.  
 
@@ -93,3 +143,213 @@ Section BindCtxUnary.
           (fun k => _) (bind t |}.
    *)
 End BindCtxUnary.
+
+Section AGIndLemma.
+  Context {E: Type} {HE: Encode E} {X: Type}.
+  Notation MP := (rel (ctree E X) (World E)). 
+  
+  (*| [t,w |= AG φ] is semantic and equivalent to [gfp AGCoindF φ t w] |*)
+  Inductive AGCoindF (R: MP -> MP) (φ: MP): ctree' E X -> World E -> Prop :=
+  | AGCoindTau: forall u w,
+      not_done w ->
+      R φ u w ->
+      φ (Tau u) w ->
+      AGCoindF R φ (TauF u) w
+  | AGCoindVis: forall w e k (_: encode e),
+      not_done w ->
+      (forall (v: encode e), R φ (k v) (Obs e v)) ->
+      φ (Vis e k) w ->
+      AGCoindF R φ (VisF e k) w
+  | AGCoindBr: forall n w k,
+      not_done w ->
+      (forall (i: fin' n), R φ (k i) w) ->
+      φ (Br n k) w ->
+      AGCoindF R φ (BrF n k) w.
+  Hint Constructors AGCoindF: ctl.
+
+  Program Definition agcoind_: mon (MP -> MP) :=
+    {| body R φ t w := AGCoindF R φ (observe t) w |}. 
+  Next Obligation.
+    unfold pointwise_relation, Basics.impl, Proper, respectful.
+    cbn; intros; dependent induction H0; rewrite <- x; auto with ctl.
+  Qed.
+
+  Definition agcoind: MP -> MP := gfp (agcoind_).
+  
+End AGIndLemma.
+
+Ltac fold_agcoind_in H:=
+  multimatch type of H with
+  | context[gfp (@agcoind_ ?E ?HE ?X ?RR)] =>
+      fold (@agcoind E HE X RR) in H
+  end.
+
+Ltac fold_agcoind :=
+  match goal with
+  | |- context[gfp (@agcoind_ ?E ?HE ?X ?RR)] =>
+      fold (@agcoind E HE X RR)
+  end.
+
+Ltac __coinduction_agcoind R H :=
+  unfold agcoind; apply_coinduction; intros R H.
+
+Ltac __step_agcoind := unfold agcoind; step; fold_agcoind.
+
+#[global] Tactic Notation "step" := __step_agcoind || step.
+
+#[global] Tactic Notation "coinduction" simple_intropattern(R) simple_intropattern(H) :=
+  __coinduction_agcoind R H.
+
+Ltac __step_agcoind_in H := unfold agcoind in H; step in H; fold_agcoind_in H.
+
+#[global] Tactic Notation "step" "in" ident(H) :=
+  __step_agcoind_in H || step in H.
+
+Global Instance proper_equ_agcoind `{Encode E} {X} (φ: ctree E X -> World E -> Prop)
+  {HP: Proper (equ eq ==> eq ==> iff) φ}:
+  Proper (equ eq ==> eq ==> iff) (agcoind φ).
+Proof.
+  unfold Proper, respectful.
+  split; subst; revert y0; generalize dependent y;  generalize dependent x;
+  coinduction R CIH; intros. 
+  - (* -> *) desobs y; observe_equ Heqt;
+               rewrite Eqt in H0; step in H0; cbn in H0; dependent destruction H0;
+               step in H1; cbn in H1; do 3 red; cbn.
+    + (* Ret *)
+      rewrite <- x in H1.
+      inv H1.
+    + (* Br *)
+      rewrite Heqt.
+      rewrite <- x in H1.
+      dependent destruction H1.
+      assert (HeqBr: Br n k1 ≅ Br n k) by (step; cbn; auto).
+      rewrite HeqBr in H3.
+      eapply AGCoindBr; auto.
+      intro i.
+      specialize (H0 i).
+      eapply CIH with (k1 i); auto.
+    + (* Vis *)
+      rewrite Heqt.
+      rewrite <- x in H1.
+      inv H1.
+      apply AGCoindTau; auto.
+      eapply CIH with t1; eauto.
+      assert (HeqTau: Tau t1 ≅ Tau t) by (step; cbn; auto).
+      now rewrite <- HeqTau.
+    + rewrite Heqt.
+      rewrite <- x in H1.
+      dependent destruction H1.
+      assert (HeqVis: Vis e k1 ≅ Vis e k) by (step; cbn; auto).
+      rewrite HeqVis in H3.
+      eapply AGCoindVis; auto.
+      intro v.
+      specialize (H0 v).
+      eapply CIH with (k1 v); auto.
+  - (* <- *)  desobs x; observe_equ Heqt;
+               rewrite Eqt in H0; step in H0; cbn in H0; dependent destruction H0;
+               step in H1; cbn in H1; do 3 red; cbn.
+    + rewrite <- x in H1.
+      inv H1.
+    + rewrite Heqt.
+      rewrite <- x in H1.
+      dependent destruction H1.
+      assert (HeqBr: Br n k ≅ Br n k2) by (step; cbn; auto).
+      rewrite <- HeqBr in H3.
+      eapply AGCoindBr; auto.
+      intro i.
+      specialize (H0 i).
+      eapply CIH with (k2 i); auto.
+    + rewrite Heqt.
+      rewrite <- x in H1.
+      inv H1.
+      apply AGCoindTau; auto.
+      eapply CIH with t2; eauto.
+      assert (HeqTau: Tau t ≅ Tau t2) by (step; cbn; auto).
+      now rewrite HeqTau.
+    + rewrite Heqt.
+      rewrite <- x in H1.
+      dependent destruction H1.
+      assert (HeqVis: Vis e k ≅ Vis e k2) by (step; cbn; auto).
+      rewrite <- HeqVis in H3.
+      eapply AGCoindVis; auto.
+      intro v.
+      specialize (H0 v).
+      eapply CIH with (k2 v); auto.
+Qed.
+
+Section AGCoindProof.
+  Context {E: Type} {HE: Encode E} {X: Type}.
+  Notation MP := (rel (ctree E X) (World E)).
+
+  Lemma ag_agcoind: forall (t: ctree E X) w φ
+                      {HP: Proper (equ eq ==> eq ==> iff) φ}
+                      {Hφ: forall t w, φ (Tau t) w <-> φ t w},
+      car φ (fun _ _ => False) t w -> agcoind φ t w.
+  Proof.
+    coinduction R CIH.
+    intros.
+    step in H.
+    do 3 red; cbn.
+    inv H; try contradiction.
+    destruct H1 as ((t' & w' & TR) & H).
+    cbn in TR, H.
+    rewrite ctree_eta in H0.
+    remember (observe t) as T.
+    remember (observe t') as T'.
+    clear HeqT t HeqT' t'.
+    induction TR.
+    - (* Tau *)
+      apply AGCoindTau; auto.
+      + now apply ktrans_not_done with t t' w'.
+      + apply CIH; auto.
+        step; apply RStepA.
+        * now apply Hφ.
+        * split. 
+          -- now (exists t', w').
+          -- intros t_ w_ TR_; auto.
+    - (* Br *)
+      apply AGCoindBr; auto.
+      intro j.
+      apply CIH; auto.
+      now apply H; econstructor.
+    - (* Vis *)
+      apply AGCoindVis; auto.
+    - (* Done *)
+      assert (TR: [Ret x, Pure] ↦ [stuck, Done x]) by now constructor.
+      specialize (H stuck (Done x) TR).
+      step in H; cbn in H.
+      dependent destruction H; try contradiction.
+      destruct H2 as ((t' & w' & TR') & H').
+      now apply ktrans_stuck in TR'.
+    - (* Finish *)
+      assert (TR: [Ret x, Obs e v] ↦ [stuck, Finish e v x]) by now constructor.
+      specialize (H stuck (Finish e v x) TR).
+      step in H; cbn in H.
+      dependent destruction H; try contradiction.
+      destruct H2 as ((t' & w' & TR') & H').
+      now apply ktrans_stuck in TR'.
+  Qed.
+  
+  Lemma ag_bind_l{Y}: forall (t: ctree E X) w (k: X -> ctree E Y) φ,
+    <( t, w |= AG now φ )> ->
+    <( {x <- t ;; k x} , w |= AG now φ )>.
+  Proof.
+    cbn.
+    coinduction R CIH.
+    intros.
+    apply ag_agcoind in H; auto with typeclass_instances.
+    step in H; cbn in H; dependent destruction H.
+    - (* Tau *)
+      apply RStepA; auto.
+      split.
+      + eapply can_step_bind_l with (w':=w); auto.
+        admit.
+      + intros t' w' TR'.
+        apply ktrans_bind_inv in TR' as
+            [(t_ & TR & Hd & Hequ) | [(v & TR & ? & ?) | (e' & v' & x' & TR & -> & TR')]].
+        * rewrite Hequ.
+          apply CIH; auto.
+          cbn in TR.
+          rewrite <- x in TR.
+          apply ktrans_tau in TR.
+          step in H0; cbn in H0; inv H0.
